Test HKDF using the vectors in RFC 5869

src/tls/HKDF.fst
@@ -5,6 +5,9 @@ open TLSConstants
 
 module CC = CoreCrypto
 
+private let max (a:int) (b:int) = if a < b then b else a
+
+(*-------------------------------------------------------------------*)
 (*
 From https://tools.ietf.org/html/rfc5869
 
@@ -20,7 +23,16 @@ HKDF-Extract(salt, IKM) -> PRK
       PRK      a pseudorandom key (of HashLen octets)
 
    PRK = HMAC-Hash(salt, IKM)
+*)
 
+val hkdf_extract: ha:CC.hash_alg -> salt:bytes -> ikm:bytes
+  -> Tot (lbytes (CC.hashSize ha))
+
+let hkdf_extract ha salt ikm = CC.hmac ha salt ikm
+
+
+(*-------------------------------------------------------------------*)
+(*
 HKDF-Expand(PRK, info, L) -> OKM
    Options:
       Hash     a hash function; HashLen denotes the length of the
@@ -46,15 +58,7 @@ HKDF-Expand(PRK, info, L) -> OKM
    ...
 *)
 
-private let max (a:int) (b:int) = if a < b then b else a
-
-val hkdf_extract: ha:CC.hash_alg -> salt:bytes -> ikm:bytes
-  -> Tot (lbytes (CC.hashSize ha))
-
-let hkdf_extract ha salt ikm = CC.hmac ha salt ikm
-
-
-val hkdf_expand_int: ha:CC.hash_alg
+private val hkdf_expand_int: ha:CC.hash_alg
   -> prk:bytes{CC.hashSize ha <= length prk}
   -> info:bytes
   -> len:nat{len <= op_Multiply 255 (CC.hashSize ha)}
@@ -73,22 +77,56 @@ let rec hkdf_expand_int ha prk info len count curr prev =
     prev @| next
   else empty_bytes
 
+val hkdf_expand: ha:CoreCrypto.hash_alg
+  -> prk:bytes{CC.hashSize ha <= length prk}
+  -> info:bytes
+  -> len:nat{len <= op_Multiply 255 (CC.hashSize ha)}
+  -> Tot (lbytes len)
+
+let hkdf_expand ha prk info len =
+  lemma_repr_bytes_values len;
+  let res = hkdf_expand_int ha prk info len 0 0 empty_bytes in
+  let sp1,_ = split res len in
+  sp1
+
+
+(*-------------------------------------------------------------------*)
+(*
+HKDF-Expand-Label(Secret, Label, Messages, Length) =
+       HKDF-Expand(Secret, HkdfLabel, Length)
+
+  Where HkdfLabel is specified as:
+
+  struct HkdfLabel {
+    uint16 length;
+    opaque label<9..255>;
+    opaque hash_value<0..255>;
+  };
+
+  - HkdfLabel.length is Length
+  - HkdfLabel.label is "TLS 1.3, " + Label
+  - HkdfLabel.hash_value is HashValue.
+*)
+
+val tls13_prefix: lbytes 9
+let tls13_prefix =
+  let s = abytes "TLS 1.3, " in
+  assume (length s = 9); // Cannot be proved because abytes is underspecified
+  s
 
 val hkdf_expand_label: ha:CoreCrypto.hash_alg
   -> prk:bytes{CC.hashSize ha <= length prk}
-  -> label:string{length (abytes ("TLS 1.3, " ^ label)) < 256}
+  -> label:string{length (abytes label) < 256 - 9}
   -> hv:bytes{length hv < 256}
   -> len:nat{len <= op_Multiply 255 (CC.hashSize ha)}
   -> Tot (lbytes len)
 
 let hkdf_expand_label ha prk label hv len =
-  let label_bytes = abytes ("TLS 1.3, " ^ label) in
-  lemma_repr_bytes_values (length (label_bytes));
+  let label_bytes = tls13_prefix @| abytes label in
   lemma_repr_bytes_values len;
+  lemma_repr_bytes_values (length (label_bytes));
   lemma_repr_bytes_values (length hv);
   let info = (bytes_of_int 2 len) @| 
 	     (vlbytes 1 label_bytes) @|
 	     (vlbytes 1 hv) in
-  let res = hkdf_expand_int ha prk info len 0 0 empty_bytes in
-  let sp1,_ = split res len in
-  sp1
+  hkdf_expand ha prk info len
